rename constant

WPDS/WPDS_Code.thy
@@ -19,10 +19,10 @@ definition "augmented_WPDS_rules = WPDS_with_W_automata_no_assms.\<Delta>\<^sub>
 
 definition "pre_star_exec' = WPDS_with_W_automata_no_assms.pre_star_exec'"
 
-definition "accept_pre_star_exec0' = WPDS_with_W_automata_no_assms.accept_pre_star_exec0'"
+definition "language_pre_star_exec0' = WPDS_with_W_automata_no_assms.language_pre_star_exec0'"
 
 context fixes finals :: "('ctr_loc, 'noninit) state set" begin
-abbreviation accepts ("\<L>(_)" [1000] 1000) where "\<L>(ts') \<equiv> dioidLTS.accepts ts' finals"
+abbreviation language ("\<L>(_)" [1000] 1000) where "\<L>(ts') \<equiv> dioidLTS.language ts' finals"
 lemma pre_star_exec_correctness:
   assumes "checking"
   shows "\<L>(WPDS_with_W_automata_no_assms.pre_star_exec' (set \<Delta>) ts) (Init p, w) =
@@ -53,9 +53,9 @@ definition run_WPDS_reach ::
  "run_WPDS_reach \<Delta> ts ts' = run_WPDS_reach' \<Delta> (ts_to_wts ts) (ts_to_wts ts')"
 
 declare WPDS_Code.checking_def[code]
-declare WPDS_Code.accept_pre_star_exec0'_def[code]
+declare WPDS_Code.language_pre_star_exec0'_def[code]
 declare WPDS.lbl.simps[code]
-declare WPDS.accept_pre_star_exec0_def[code]
+declare WPDS.language_pre_star_exec0_def[code]
 declare Enum.enum_class.UNIV_enum[code]
 
 
@@ -69,14 +69,14 @@ interpretation finite_WPDS "(set \<Delta>)"
 interpretation countable_dioidLTS transition_rel apply standard
   using countable_transition_rel .
 
-lemma weight_reach_set'_lang_aut_is_weight_reach'_accepts_full:
+lemma weight_reach_set'_lang_aut_is_weight_reach'_language_full:
   fixes ts :: "(('ctr_loc, 'noninit::enum) state, 'label) transition set"
   fixes ts' :: "(('ctr_loc, 'noninit) state, 'label) transition set"
   assumes "finite ts"
   assumes "finite ts'"
   shows "weight_reach_set (P_Automaton.lang_aut ts Init finals) (P_Automaton.lang_aut ts' Init finals') =
-         weight_reach (accepts_full (ts_to_wts ts) finals) (accepts_full (ts_to_wts ts') finals')"
-  unfolding lang_aut_is_accepts_full[OF assms(1)] lang_aut_is_accepts_full[OF assms(2)]
+         weight_reach (language_full (ts_to_wts ts) finals) (language_full (ts_to_wts ts') finals')"
+  unfolding lang_aut_is_language_full[OF assms(1)] lang_aut_is_language_full[OF assms(2)]
   using weight_reach_set_is_weight_reach by blast
 
 lemma WPDS_reach_exec_correct:
@@ -89,12 +89,12 @@ proof -
     using assms unfolding run_WPDS_reach_def run_WPDS_reach'_def
     by (metis (no_types, lifting) option.distinct(1))
   then have "weight_reach_sum_exec \<lbrakk>(ts_to_wts ts) \<inter>\<^sub>w (WPDS_with_W_automata_no_assms.pre_star_exec' (set \<Delta>) (ts_to_wts ts'))\<rbrakk>\<^sub>w {(p, p) |p. p \<in> inits_set} (finals \<times> finals')
-        = weight_reach (accepts_full (ts_to_wts ts) finals) (accepts_full (ts_to_wts ts') finals')"
+        = weight_reach (language_full (ts_to_wts ts) finals) (language_full (ts_to_wts ts') finals')"
     using WPDS_weight_reach'_is_weight_reach_sum_exec[of "ts_to_wts ts" "ts_to_wts ts'" inits_set finals finals', OF binary_aut_ts_to_wts[of ts]]
     unfolding inits_set_def mem_Collect_eq WPDS_Code.checking_def
     by simp
   then show ?thesis
-    unfolding weight_reach_set'_lang_aut_is_weight_reach'_accepts_full[of ts ts' finals finals', unfolded finite_code, simplified]
+    unfolding weight_reach_set'_lang_aut_is_weight_reach'_language_full[of ts ts' finals finals', unfolded finite_code, simplified]
     using assms unfolding run_WPDS_reach_def run_WPDS_reach'_def
     by (metis (lifting) option.distinct(1) option.inject)
 qed
